Compilation now produces actual facade modules.
Star working on cleaning up the automation, prove lemmas to connect
Facade's preconditions to ours, to convert Facade's environments into
ours, and to adjust the output of our compiler into a format suitable
for the Facade compiler.

examples/FiniteSetsExamples.v
@@ -1,9 +1,6 @@
 (** * Some examples about dealing with finite sets *)
 Require Import ADTSynthesis.FiniteSetADTs.
 
-(** Now we spec out two examples, the count of the unique elements in
-    a list, and the sum of the unique elements in a list. *)
-
 Definition countUniqueSpec (ls : list W) : Comp W
   := cardinal (elements ls).
 
@@ -73,37 +70,10 @@ Require Import Computation.ApplyMonad.
 Require Import GLabelMapFacts.
 Require Import List.
 Require Import FiniteSetADTs.FiniteSetADTMethodLaws.
+Require Import FiatToFacade.Compiler.Automation.Vacuum.
 
-Ltac find_label_in_env :=
-  unfold basic_env, AddPair, MakePair; simpl;
-  try match goal with
-        | |- GLabelMap.find ?k (GLabelMap.add ?k' (Axiomatic ?spec) _) = Some (Axiomatic ?spec) =>
-          apply P.F.add_eq_o; try reflexivity
-        | |- GLabelMap.find ?k (GLabelMap.add ?k' (Axiomatic ?spec) _) = Some (Axiomatic ?spec') =>
-          rewrite P.F.add_neq_o; [ find_label_in_env | ]; congruence
-      end.
-
-Ltac vacuum :=
-  trickle_deletion;
-  match goal with
-    | [ |- refine _ _ ] => try (simplify with monad laws)
-    | [ |- ?a <> ?b ] => first [ is_evar a | is_evar b | discriminate ]
-    | [ |- ~ StringMap.In ?k ∅ ] => solve [apply not_in_empty]
-    | [ |- ~ StringMap.In ?k ?s ] => first [ is_evar s | solve [map_iff_solve ltac:(intuition discriminate)] ]
-    | [ |- context[SCALoopBodyProgCondition] ] => progress (unfold SCALoopBodyProgCondition; intros; simpl)
-    | [ |- context[ADTLoopBodyProgCondition] ] => progress (unfold ADTLoopBodyProgCondition; intros; simpl)
-    | [ |- context[PairLoopBodyProgCondition] ] => progress (unfold PairLoopBodyProgCondition; intros; simpl)
-    | [ |- ?m[?k >> ?v] ] => solve [map_iff_solve_evar intuition]
-    | [ |- SomeSCAs _ ∅ ] => solve [apply SomeSCAs_empty]
-    | [ |- SomeSCAs _ _ ] => eassumption
-    | [ |- AllADTs _ _ ] => eassumption
-    | [ |- AllADTs _ _ ] => solve [unfold AllADTs, Superset; intros; map_iff_solve intuition]
-    | [ |- Word2Spec ?env _ = Some (Axiomatic _) ] => reflexivity
-    | [ |- Label2Word ?env _ = Some _ ] => reflexivity
-    | [ |- StringMap.Equal ?a ?b ] => first [ is_evar a | is_evar b | trickle_deletion; reflexivity ]
-    | [ |- Core.AbsR ?impl ?e (projT1 ?fs) ] => exact (proj2_sig (projT2 fs))
-    | _ => solve [ find_label_in_env ]
-  end.
+(** Now we spec out two examples, the count of the unique elements in
+    a list, and the sum of the unique elements in a list. *)
 
 (*
 
@@ -253,111 +223,100 @@ Defined.
 *)
 (** And now we do the same for summing. *)
 
-Notation FullySharpenedFacadeProgramOnListReturningWord spec ls
-  := (sig (fun p => refine (x <- spec;
-                            @Prog _ basic_env True ∅
-                                  (["$ret" >sca> x]::∅)
-                                  (["$ls" >adt> List ls]::∅)
-                                  ∅)
-                           (ret p))).
+Require Import Facade.CompileDFacade.
+Require Import CompileUnit.
+Require Import Compiler.Automation.FacadeHelpers.
+Require Import Compiler.Automation.SpecializedFolds.
+
+Definition ProgramOnListReturningWord_pre :=
+  (fun v1 v2 => exists ls w, v1 = ADT (List ls) /\ v2 = SCA ADTValue w).
+
+Definition ProgramOnListReturningWord_post spec :=
+  (fun v1 v2 retval => exists ls w wret, v1 = ADT (List ls) /\ v2 = SCA ADTValue w /\
+                                         retval = SCA ADTValue wret /\ computes_to (spec ls) wret).
+
+Definition ProgramOnListReturningWord_refinement spec ls retval prog :=
+  refine (r <- spec ls;
+          p <- (@Prog ADTValue basic_imports_wrapped True ∅
+                      ([retvar >sca> r]::∅)
+                      ([argvar1 >adt> List ls]::∅)
+                      ∅);
+          ret (r, p))
+         (ret (retval, prog)).
+
+Lemma FullySharpenedFacadeProgramOnListReturningWordByRefinements spec P :
+  (sigT (fun prog =>
+           (forall ls, exists retval,
+              ProgramOnListReturningWord_refinement spec ls retval prog)
+           /\ P prog)) ->
+  (sigT (fun prog => PairOfConditionsForCompileUnit _ prog
+                                                    ProgramOnListReturningWord_pre
+                                                    (ProgramOnListReturningWord_post spec)
+                                                    basic_imports
+                     /\ P prog)).
+Proof.
+  unfold PairOfConditionsForCompileUnit, ProgramOnListReturningWord_refinement,
+         ProgramOnListReturningWord_pre, ProgramOnListReturningWord_post, Prog.
+  intros [ prog (forall_ls & ?) ].
+  exists prog; split; [ | assumption ]; apply two_conds_as_one; intros st v1 v2 map_eq [ls [w (sv1 & sv2)]]; subst;
+  cbv delta [StringMapFacts.make_map] in *; simpl in *;
+  specialize (forall_ls ls); destruct forall_ls as [retval refi].
+
+  apply pick_compile_helper in refi.
+  destruct refi as (retval_correct & prog_ok); hnf in prog_ok.
+
+  match type of (prog_ok st) with
+    | ?a /\ ?b /\ ?c -> _ =>
+      assert a by apply I; assert b; assert c;
+      try rewrite map_eq;
+      first [ eapply AllADTs_chomp, add_adts_pop_sca; map_iff_solve intuition
+            | apply SomeSCAs_empty
+            | specialize_states; split; try solve [ intuition ] ]
+  end.
+
+  intros; destruct_pairs; specialize_states.
+
+  exists (SCA ADTValue retval).
+  split; intros; destruct_pairs.
+
+  scas_adts_mapsto;
+  unfold StringMapFacts.Submap;
+  setoid_rewrite <- StringMapFacts.find_mapsto_iff; intros *;
+  map_iff_solve intuition.
+
+  split;
+    [ destruct_pairs;
+      intros; eapply not_in_adts_not_mapsto_adt; eauto;
+      try apply not_in_empty
+    | repeat eexists; repeat split; first [ reflexivity | eassumption ] ].
+Qed.       
+
+Definition FullySharpenedFacadeProgramOnListReturningWord spec :=
+  CompileUnit ProgramOnListReturningWord_pre (ProgramOnListReturningWord_post spec).
+
+Lemma CompileUnit_construct av pre_cond post_cond imports:
+  (sigT (fun prog =>
+           PairOfConditionsForCompileUnit av prog pre_cond post_cond imports /\
+           (is_disjoint (assigned prog) (StringSetFacts.of_list argvars) = true /\
+            is_syntax_ok prog = true)) ->
+   CompileUnit pre_cond post_cond).
+Proof.
+  intros [ prog ((? & ?) & ? & ?) ].
+  econstructor; eauto.
+Qed.
 
 Tactic Notation "begin" "sharpening" "facade" "program" :=
-  (lazymatch goal with
-  | [ |- sig (fun p => refine (x <- ?spec; @Prog _ _ _ _ _ _ _) (ret p)) ]
-    => (let T := match type of spec with Comp ?T => constr:T end in
-        let c := fresh in
-        evar (c : T);
-        let H := fresh in
-        assert (H : refine spec (ret c)); subst c;
-        [
-        | eexists; rewrite H; simplify with monad laws ])
-  | [ |- ?G ] => fail "Goal is not about sharpening a facade program." "Goal:" G "is not of the form" "{ p : _ | refine (x <- spec; Prog _ _ _ _ _) (ret p) }"
-   end).
+  idtac;
+  (match goal with
+     | [ |- FullySharpenedFacadeProgramOnListReturningWord ?spec ] =>
+       (unfold FullySharpenedFacadeProgramOnListReturningWord;
+        apply (CompileUnit_construct (imports := basic_imports));
+        apply FullySharpenedFacadeProgramOnListReturningWordByRefinements;
+        econstructor; split; [ intro; eexists; unfold ProgramOnListReturningWord_refinement | ])
+     | [ |- ?G ] => fail "Goal is not about sharpening a facade program."
+                         "Goal:" G "is not of the form" "FullySharpenedFacadeProgramOnListReturningWord _"
+  end).
   
-Lemma compile_FiniteSetAndFunctionOfList_SCA (FiniteSetImpl : FullySharpened FiniteSetSpec)
-      f (x : W) ls
-      tis_empty thead vadt {vret}
-      flistrev flistempty flistpop fsetempty fsetdelete
-      {env}
-      {vls} (vdiscard: StringMap.key)
-      init_knowledge
-      init_scas init_adts
-:
-  GLabelMap.find (elt:=FuncSpec ADTValue) flistrev env = Some (Axiomatic List_rev) ->
-  GLabelMap.find (elt:=FuncSpec ADTValue) flistempty env = Some (Axiomatic List_empty) ->
-  GLabelMap.find (elt:=FuncSpec ADTValue) flistpop env = Some (Axiomatic List_pop) ->
-  GLabelMap.find (elt:=FuncSpec ADTValue) fsetempty env = Some (Axiomatic FEnsemble_sEmpty) ->
-  GLabelMap.find (elt:=FuncSpec ADTValue) fsetdelete env = Some (Axiomatic FEnsemble_sDelete) ->
-  vret <> vadt ->
-  vret <> vls ->
-  vret <> tis_empty ->
-  vadt <> vls ->
-  vadt <> tis_empty ->
-  thead <> vret ->
-  thead <> vadt ->
-  thead <> vls ->
-  vls <> vret ->
-  tis_empty <> vls ->
-  vls <> vdiscard ->
-  ~ StringMap.In vadt init_adts ->
-  ~ StringMap.In vret init_adts ->
-  ~ StringMap.In thead init_adts ->
-  ~ StringMap.In tis_empty init_adts ->
-  ~ StringMap.In vdiscard init_adts ->
-  ~ StringMap.In vdiscard init_scas ->
-  ~ StringMap.In vadt init_scas ->
-  ~ StringMap.In vls init_scas ->
-  ~ StringMap.In tis_empty init_scas ->
-  refine (@Prog _ env init_knowledge
-                init_scas ([vret >sca> (snd (FiniteSetAndFunctionOfList FiniteSetImpl f x ls))] :: init_scas)
-                ([vls >adt> List ls]::init_adts)
-                ([vls >adt> List nil]::init_adts))
-         (cloop <- { cloop : Stmt
-                    | PairLoopBodyOk
-                        basic_env
-                        (fun xs_acc w =>
-                           ValidFiniteSetAndFunctionOfList_body
-                             FiniteSetImpl
-                              f
-                             w
-                             xs_acc)
-                        cloop init_knowledge init_scas init_adts vls vret vadt thead tis_empty snd
-                        (fun xs_acc =>
-                           FEnsemble (to_ensemble FiniteSetImpl (projT1 (fst xs_acc)))) };
-          ret
-            (Seq
-               (Seq (Call vdiscard flistrev (cons vls nil))
-                    (Seq (Assign vret (Const x))
-                         (Seq (Call vadt fsetempty nil)
-                              (Fold thead tis_empty vls flistpop flistempty cloop))))
-               (Call tis_empty fsetdelete (cons vadt nil)))).
-Proof.
-  intros.
-  rewrite FiniteSetAndFunctionOfList_ValidFiniteSetAndFunctionOfList.
-  unfold ValidFiniteSetAndFunctionOfList.
-  rewrite <- (@rev_involutive _ ls).
-  rewrite !fold_left_rev_right.
-  rewrite -> (@rev_involutive _ ls).
-  simpl.
-  
-  rewrite (compile_pair_sca vadt (fun x => FEnsemble (to_ensemble _ (projT1 (fst x))))); vacuum.
-
-  rewrite (fun b => @compile_list_rev_general env flistrev vdiscard vls b _ _ _); try first [ eassumption | rewrite add_add_add'; reflexivity | vacuum ].
-
-  rewrite add_add_add'.
-  setoid_rewrite (compile_fold_pair env _ snd (fun x => FEnsemble (to_ensemble _ (projT1 (fst x)))) vls vret vadt thead tis_empty flistpop flistempty); try first [ eassumption | solve [map_iff_solve intuition] | vacuum ].
-
-  simpl.
-  unfold W.
-  rewrite General.refine_under_bind (* Apply should work here *).
-
-  Focus 2.
-  intros.
-  rewrite compile_constant; vacuum.
-  rewrite compile_AbsImpl_sEmpty; first [ eassumption | solve [map_iff_solve eauto] | vacuum ]. 
-  rewrite compile_AbsImpl_sDelete; try first [ eassumption | solve [map_iff_solve eauto] | vacuum ].
-Admitted.
-
 Lemma eq_ToEnsemble_In (FiniteSetImpl: FullySharpened FiniteSetSpec)
       (st : { st : _ & { S0 : _ | Core.AbsR (projT2 FiniteSetImpl) S0 st }%type})
       key
@@ -371,53 +330,6 @@ Proof.
   apply Same_set_ToEnsemble_AbsR; trivial.
   apply AbsR_ToEnsemble_In; trivial.
 Qed.
-
-
-Lemma compile_list_delete_no_ret :
-  forall vret vseq env f seq knowledge scas adts adts',
-    GLabelMap.find f env = Some (Axiomatic List_delete) ->
-    ~ StringMap.In vret adts ->
-    ~ StringMap.In vret scas ->
-    ~ StringMap.In vseq scas ->
-    adts[vseq >> ADT (List seq)] ->
-    StringMap.Equal adts' (StringMap.remove vseq adts) ->
-    refine (@Prog _ env knowledge
-                  scas scas
-                  adts adts')
-           (ret (Call vret f (vseq :: nil)))%facade.
-Proof.
-  compile_list_helper runsto_delete.
-
-  eauto using SomeSCAs_chomp_left, SomeSCAs_chomp, SomeSCAs_not_In_remove.
-  
-  apply add_adts_pop_sca.
-  map_iff_solve intuition.
-  eauto using AllADTs_chomp_remove'.
-Qed.
-
-(*
-Lemma compile_list_delete_no_return
-      (vret : StringMap.key)
-      (env : GLabelMap.t (FuncSpec ADTValue))
-      (f : GLabelMap.key) (vseq : StringMap.key)
-      (seq : list Memory.W) (knowledge : Prop)
-      (scas adts : StringMap.t (Value ADTValue))
-: GLabelMap.find (elt:=FuncSpec ADTValue) f env =
-  Some (Axiomatic List_delete) ->
-  ~ StringMap.In (elt:=Value ADTValue) vret adts ->
-  ~ StringMap.In (elt:=Value ADTValue) vseq adts ->
-  ~ StringMap.In (elt:=Value ADTValue) vseq scas ->
-  ~ StringMap.In (elt:=Value ADTValue) vret scas ->
-  vret <> vseq ->
-  refine
-    (Prog (env := env) knowledge scas scas ([vseq >> ADT (List seq)]::adts) adts)
-    (Return (Call vret f (cons vseq nil))).
-Proof.
-  intros.
-  eapply compile_list_delete_no_ret; eauto; try vacuum.
-  (* Same as compile_list_delete_no_ret ?*)
-Admitted.
-*)
 
 Ltac new_variable_name base :=
   let base' := (eval compute in base) in
@@ -489,48 +401,6 @@ Ltac solve_SomeSCAs :=
                   end
            end) ].
 
-
-
-(*Ltac get_post_prog_and_var_from G :=
-  (lazymatch G with
-  | refine (prog <- { prog : _ | ProgOk prog _ _ ([?var >> SCA _ ?p]::_) _ _ }; _) _ => constr:((var, p))
-  | refine ({ prog : _ | ProgOk prog _ _ ([?var >> SCA _ ?p]::_) _ _ }) _ => constr:((var, p))
-   end).
-Ltac get_post_prog_and_var_in_goal :=
-  let G := match goal with |- ?G => constr:G end in
-  get_post_prog_and_var_from G.
-
-Ltac get_post_adt_and_var_from G :=
-  (lazymatch G with
-  | refine (prog <- { prog : _ | ProgOk prog _ _ _ _ ([?var >> ADT ?p]::_) }; _) _ => constr:((var, p))
-  | refine ({ prog : _ | ProgOk prog _ _ _ _ ([?var >> ADT ?p]::_) }) _ => constr:((var, p))
-   end).
-
-Ltac get_post_adt_and_var_in_goal :=
-  let G := match goal with |- ?G => constr:G end in
-  get_post_adt_and_var_from G.
-
-
-
-Ltac get_pre_prog_and_var_from G :=
-  (lazymatch G with
-  | refine (prog <- { prog : _ | ProgOk prog _ ([?var >> SCA _ ?p]::_) _ _ _ }; _) _ => constr:((var, p))
-  | refine ({ prog : _ | ProgOk prog _ ([?var >> SCA _ ?p]::_) _ }) _ _ _ => constr:((var, p))
-   end).
-Ltac get_pre_prog_and_var_in_goal :=
-  let G := match goal with |- ?G => constr:G end in
-  get_pre_prog_and_var_from G.
-
-Ltac get_pre_adt_and_var_from G :=
-  (lazymatch G with
-  | refine (prog <- { prog : _ | ProgOk prog _ _ _ ([?var >> ADT ?p]::_) _ }; _) _ => constr:((var, p))
-  | refine ({ prog : _ | ProgOk prog _ _ _ ([?var >> ADT ?p]::_) _ }) _ => constr:((var, p))
-   end).
-
-Ltac get_pre_adt_and_var_in_goal :=
-  let G := match goal with |- ?G => constr:G end in
-  get_pre_adt_and_var_from G.*)
-
 Ltac guarded_compile_step_same_states :=
   idtac;
   let p := get_pre_post_scas_adts_from_goal in
@@ -587,7 +457,8 @@ Ltac compile_step_same_adts_handle_first_post_sca :=
           => (let tis_empty := new_variable_name "$is_empty" in
               let thead     := new_variable_name "$head" in
               let vadt      := new_variable_name "$adt" in
-              let lem       := constr:(@compile_FiniteSetAndFunctionOfList_SCA impl f x ls tis_empty thead vadt var) in
+              let vdiscard  := new_variable_name "$discard" in
+              let lem       := constr:(@compile_FiniteSetAndFunctionOfList_SCA impl f x ls tis_empty thead vadt vdiscard var) in
               first [ rewrite lem
                     | setoid_rewrite lem ])
         | if _ then _ else _
@@ -685,21 +556,20 @@ Ltac compile_step :=
 
 Tactic Notation "compile" := repeat repeat compile_step.
 
-Tactic Notation "finish" "compiling" := reflexivity.
+Tactic Notation "finish" "compiling" := (split; reflexivity). 
 
-Definition sumUniqueImpl (FiniteSetImpl : FullySharpened FiniteSetSpec) (ls : list W)
-: FullySharpenedFacadeProgramOnListReturningWord (sumUniqueSpec ls) ls.
-Proof.
+Definition sumUniqueImpl (FiniteSetImpl : FullySharpened FiniteSetSpec)
+: FullySharpenedFacadeProgramOnListReturningWord sumUniqueSpec.
+Proof.       
   begin sharpening facade program.
-
+  
   sharpen computation with FiniteSet implementation := FiniteSetImpl.
 
-  finish sharpening computation.
-
   Time compile. (* 47 s *)
-
   admit.
-Admitted.
+
+  finish compiling.
+Qed.
 
 Definition sumAllImpl (FiniteSetImpl : FullySharpened FiniteSetSpec) (ls : list W)
 : FullySharpenedComputation (sumAllSpec ls).
@@ -709,8 +579,6 @@ Proof.
   begin sharpening computation.
 
   sharpen computation with FiniteSet implementation := FiniteSetImpl.
-
-
 
   finish sharpening computation.
 Defined.
