src/FiatToFacade/Compiler.v
@@ -15,25 +15,47 @@ Require Export
         FiatToFacade.Compiler.ADTs.FiniteSets.
 
 Require Export Common.
+Require Export Cito.StringMap.
+Require Export Cito.GLabelMap.
 Require Export Facade.Facade.
 Require Export Facade.DFacade.
 Require Export Facade.examples.FiatADTs.
-Require Export Cito.StringMap.
-Require Export Cito.GLabelMap.
 
-Definition AddPair {av} pair m :=
-  @GLabelMap.add (FuncSpec av) (fst pair) (snd pair) m.
+Unset Implicit Arguments.
 
-Definition MakePair {av} (k: GLabel.glabel) (v: AxiomaticSpec av) :=
-  (k, Axiomatic v).
+Definition MakePair {elt} (k: GLabel.glabel) (v: elt) :=
+  (k, v).
+
+Definition AddPair {elt} pair m :=
+  @GLabelMap.add elt (fst pair) (snd pair) m.
 
 Notation "[[[ p1 ; .. ; pn ]]]" :=
   (AddPair p1 .. (AddPair pn (GLabelMap.empty _)) ..).
 
-Notation "k ↦ v" :=
+Notation "k ⇥ v" :=
   (MakePair k v) (at level 55, no associativity).
 
+Notation "k ↦ v" :=
+  (MakePair k (Axiomatic v)) (at level 55, no associativity).
+
 Definition empty_env {av} := GLabelMap.empty (FuncSpec av).
+
+Definition basic_imports := [[[ ("List", "Empty") ⇥ List_empty;
+                                ("List", "Pop") ⇥ List_pop;
+                                ("List", "New") ⇥ List_new;
+                                ("List", "Push") ⇥ List_push;
+                                ("List", "Copy") ⇥ List_copy;
+                                ("List", "Delete") ⇥ List_delete;
+                                ("List", "Rev") ⇥ List_rev;
+                                ("FSet", "Empty") ⇥ FEnsemble_sEmpty;
+                                ("FSet", "Add") ⇥ FEnsemble_sAdd;
+                                ("FSet", "Remove") ⇥ FEnsemble_sRemove;
+                                ("FSet", "Delete") ⇥ FEnsemble_sDelete;
+                                ("FSet", "In") ⇥ FEnsemble_sIn;
+                                ("FSet", "Size") ⇥ FEnsemble_sSize
+                              ]]].
+
+Definition basic_imports_wrapped := (GLabelMap.map (@Axiomatic _) basic_imports).
 
 Definition basic_env := [[[ ("List", "Empty") ↦ List_empty;
                             ("List", "Pop") ↦ List_pop;
@@ -41,6 +63,7 @@ Definition basic_env := [[[ ("List", "Empty") ↦ List_empty;
                             ("List", "Push") ↦ List_push;
                             ("List", "Copy") ↦ List_copy;
                             ("List", "Delete") ↦ List_delete;
+                            ("List", "Rev") ↦ List_rev;
                             ("FSet", "Empty") ↦ FEnsemble_sEmpty;
                             ("FSet", "Add") ↦ FEnsemble_sAdd;
                             ("FSet", "Remove") ↦ FEnsemble_sRemove;
@@ -49,12 +72,20 @@ Definition basic_env := [[[ ("List", "Empty") ↦ List_empty;
                             ("FSet", "Size") ↦ FEnsemble_sSize
                           ]]].
 
-Unset Implicit Arguments.
+Require Import Cito.GLabelMapFacts.
+
+Lemma basic_imports_yield_basic_env :
+  GLabelMap.Equal basic_imports_wrapped basic_env.
+Proof.
+  unfold basic_imports_wrapped, basic_imports, basic_env.
+
+  repeat (etransitivity; [ apply GLabelMapFacts.map_add | ];
+          apply GLabelMapFacts.F.add_m; try reflexivity).
+  apply map_empty.
+Qed.
 
 Definition start_adt state vret {ret_type v} wrapper wrapper_inj adts :=
   (@start_compiling_adt_with_precondition _ basic_env state ∅ adts vret ret_type v wrapper wrapper_inj).
 
 Definition start_sca state vret adts :=
   (@start_compiling_sca_with_precondition _ basic_env state ∅ adts vret).
-
-Notation refine' := refine.
