src/FiatToFacade/Compiler/Automation.v
@@ -1,0 +1,4 @@
+Require Export FiatToFacade.Compiler.
+
+Require Export FiatToFacade.Compiler.Automation.Vacuum.
+Require Export FiatToFacade.Compiler.Automation.SpecializedFolds.
