src/FiatToFacade/Compiler/Automation/FacadeHelpers.v
@@ -1,0 +1,60 @@
+Require Import CompileDFacade.
+Require Import FiatToFacade.Compiler.
+Require Import List.
+
+Notation argvar1 := "arg1".
+Notation argvar2 := "arg2".
+Notation argvars := (argvar1 :: argvar2 :: nil).
+Notation retvar := "ret".
+
+Unset Implicit Arguments.
+
+Definition PairOfConditionsForCompileUnit av prog (pre_cond: _ -> _ -> Prop) post_cond imports :=
+  (forall st value1 value2, 
+     StringMap.Equal st (StringMapFacts.make_map (argvar1 :: argvar2 :: nil) (value1 :: value2 :: nil)) -> 
+     pre_cond value1 value2 -> DFacade.Safe (GLabelMap.map (@Axiomatic av) imports) prog st) /\
+  (forall st st' value1 value2, 
+     StringMap.Equal st (StringMapFacts.make_map (argvar1 :: argvar2 :: nil) (value1 :: value2 :: nil)) -> 
+     pre_cond value1 value2 -> DFacade.RunsTo (GLabelMap.map (@Axiomatic av) imports) prog st st' -> 
+     exists ret, StringMapFacts.Submap (StringMapFacts.make_map (retvar :: nil) (ret :: nil)) st' /\
+                 (forall x, x <> retvar -> not_mapsto_adt x st' = true) /\
+                 post_cond value1 value2 ret).
+
+Lemma two_conds_as_one :
+  forall av prog (pre_cond: _ -> _ -> Prop) post_cond imports,
+  (forall st value1 value2, 
+           StringMap.Equal st (StringMapFacts.make_map (argvar1 :: argvar2 :: nil) (value1 :: value2 :: nil)) -> 
+           pre_cond value1 value2 -> 
+           DFacade.Safe (GLabelMap.map (@Axiomatic av) imports) prog st /\
+           forall st',
+             DFacade.RunsTo (GLabelMap.map (@Axiomatic av) imports) prog st st' -> 
+             exists ret, StringMapFacts.Submap (StringMapFacts.make_map (retvar :: nil) (ret :: nil)) st' /\
+                         (forall x, x <> retvar -> not_mapsto_adt x st' = true) /\
+                         post_cond value1 value2 ret)  <-> 
+  PairOfConditionsForCompileUnit av prog pre_cond post_cond imports.
+Proof.
+  split; intros.
+  
+  { split; intros st; [ | intros st']; intros v1 v2 eqm precond; [ | intros runsto]; specialize (H st v1 v2 eqm precond).
+    - intuition.
+    - destruct H as (_ & H);
+      specialize (H st' runsto);
+      destruct H; eexists; eauto. }
+  { destruct H as (safe & runsto).
+    split;
+      [ specialize (safe st value1 value2 H0 H1); intuition
+      | intros; specialize (runsto st st' value1 value2 H0 H1 H); destruct_ex; eexists; eauto ].
+  }
+Qed.
+
+Lemma pick_compile_helper :
+    forall (TR TP : Type) (R : Comp TR) (P : TP -> TR -> Prop) 
+           (retval : TR) (prog : TP),
+      refine (r <- R;
+              p <- {p : TP | P p r};
+              ret (r, p)) (ret (retval, prog)) -> R ↝ retval /\ P prog retval.
+Proof.
+  unfold refine; intros * h; subst.
+  specialize (h _ (AdditionalRefinementLemmas.eq_ret_compute _ _ _ eq_refl)).
+  inversion_by computes_to_inv; autoinj; subst; intuition.
+Qed.
