src/FiatToFacade/Compiler/Automation/SpecializedFolds.v
@@ -1,0 +1,89 @@
+Require Import FiatToFacade.Compiler.
+Require Import FiatToFacade.Compiler.Automation.Vacuum.
+Require Import FiniteSetADTs FiniteSetADTs.FiniteSetADTMethodLaws.
+Require Import List DFacade.
+
+Lemma compile_FiniteSetAndFunctionOfList_SCA (FiniteSetImpl : FullySharpened FiniteSetSpec)
+      f (x : W) ls
+      tis_empty thead vadt vdiscard {vret}
+      flistrev flistempty flistpop fsetempty fsetdelete
+      {env}
+      {vls}
+      init_knowledge
+      init_scas init_adts
+:
+  GLabelMap.find (elt:=FuncSpec ADTValue) flistrev env = Some (Axiomatic List_rev) ->
+  GLabelMap.find (elt:=FuncSpec ADTValue) flistempty env = Some (Axiomatic List_empty) ->
+  GLabelMap.find (elt:=FuncSpec ADTValue) flistpop env = Some (Axiomatic List_pop) ->
+  GLabelMap.find (elt:=FuncSpec ADTValue) fsetempty env = Some (Axiomatic FEnsemble_sEmpty) ->
+  GLabelMap.find (elt:=FuncSpec ADTValue) fsetdelete env = Some (Axiomatic FEnsemble_sDelete) ->
+  vret <> vadt ->
+  vret <> vls ->
+  vret <> tis_empty ->
+  vadt <> vls ->
+  vadt <> tis_empty ->
+  thead <> vret ->
+  thead <> vadt ->
+  thead <> vls ->
+  vls <> vret ->
+  tis_empty <> vls ->
+  vls <> vdiscard ->
+  ~ StringMap.In vadt init_adts ->
+  ~ StringMap.In vret init_adts ->
+  ~ StringMap.In thead init_adts ->
+  ~ StringMap.In tis_empty init_adts ->
+  ~ StringMap.In vdiscard init_adts ->
+  ~ StringMap.In vdiscard init_scas ->
+  ~ StringMap.In vadt init_scas ->
+  ~ StringMap.In vls init_scas ->
+  ~ StringMap.In tis_empty init_scas ->
+  refine (@Prog _ env init_knowledge
+                init_scas ([vret >sca> (snd (FiniteSetAndFunctionOfList FiniteSetImpl f x ls))] :: init_scas)
+                ([vls >adt> List ls]::init_adts)
+                ([vls >adt> List nil]::init_adts))
+         (cloop <- { cloop : Stmt
+                    | PairLoopBodyOk
+                        env
+                        (fun xs_acc w =>
+                           ValidFiniteSetAndFunctionOfList_body
+                             FiniteSetImpl
+                              f
+                             w
+                             xs_acc)
+                        cloop init_knowledge init_scas init_adts vls vret vadt thead tis_empty snd
+                        (fun xs_acc =>
+                           FEnsemble (to_ensemble FiniteSetImpl (projT1 (fst xs_acc)))) };
+          ret
+            (Seq
+               (Seq (Call vdiscard flistrev (cons vls nil))
+                    (Seq (Assign vret (Const x))
+                         (Seq (Call vadt fsetempty nil)
+                              (Fold thead tis_empty vls flistpop flistempty cloop))))
+               (Call tis_empty fsetdelete (cons vadt nil)))).
+Proof.
+  intros.
+  rewrite FiniteSetAndFunctionOfList_ValidFiniteSetAndFunctionOfList.
+  unfold ValidFiniteSetAndFunctionOfList.
+  rewrite <- (@rev_involutive _ ls).
+  rewrite !fold_left_rev_right.
+  rewrite -> (@rev_involutive _ ls).
+  simpl.
+  
+  rewrite (compile_pair_sca vadt (fun x => FEnsemble (to_ensemble _ (projT1 (fst x))))). 
+
+  rewrite (fun b => @compile_list_rev_general env flistrev vdiscard vls b _ _ _); try first [ eassumption | rewrite add_add_add'; reflexivity | vacuum ].
+
+  rewrite add_add_add'.
+  setoid_rewrite (compile_fold_pair env _ snd (fun x => FEnsemble (to_ensemble _ (projT1 (fst x)))) vls vret vadt thead tis_empty flistpop flistempty); try first [ eassumption | solve [map_iff_solve intuition] | vacuum ].
+
+  simpl.
+  unfold W.
+  apply General.refine_under_bind.
+
+  intros.
+  rewrite compile_constant; try vacuum.
+  rewrite compile_AbsImpl_sEmpty; first [ eassumption | solve [map_iff_solve eauto] | vacuum ]. 
+  rewrite compile_AbsImpl_sDelete; try first [ eassumption | solve [map_iff_solve eauto] | vacuum ].
+
+  reflexivity.
+Qed.
